Create asn namespace for Assertion

theories/Syntax/Assertions.v
@@ -31,6 +31,7 @@ From Coq Require Import
      Bool.Bool.
 From Katamaran Require Import
      Base
+     Notations
      Prelude
      Sep.Logic
      Syntax.Chunks
@@ -47,118 +48,292 @@ Module Type AssertionsOn
   (Import P : PredicateKit B)
   (Import F : FormulasOn B P)
   (Import C : ChunksOn B P).
+Module Import asn.
 
   Local Obligation Tactic := idtac.
 
   Inductive Assertion (Σ : LCtx) : Type :=
-  | asn_formula (fml : Formula Σ)
-  | asn_chunk (c : Chunk Σ)
-  | asn_chunk_angelic (c : Chunk Σ)
-  | asn_if   (b : Term Σ ty.bool) (a1 a2 : Assertion Σ)
-  | asn_match_enum (E : enumi) (k : Term Σ (ty.enum E)) (alts : forall (K : enumt E), Assertion Σ)
-  | asn_match_sum (σ τ : Ty) (s : Term Σ (ty.sum σ τ)) (xl : LVar) (alt_inl : Assertion (Σ ▻ xl∷σ)) (xr : LVar) (alt_inr : Assertion (Σ ▻ xr∷τ))
-  | asn_match_list
+  | formula (fml : Formula Σ)
+  | chunk (c : Chunk Σ)
+  | chunk_angelic (c : Chunk Σ)
+  | match_bool (b : Term Σ ty.bool) (A1 A2 : Assertion Σ)
+  | match_enum (E : enumi) (k : Term Σ (ty.enum E)) (alts : forall (K : enumt E), Assertion Σ)
+  | match_sum (σ τ : Ty) (s : Term Σ (ty.sum σ τ)) (xl : LVar) (alt_inl : Assertion (Σ ▻ xl∷σ)) (xr : LVar) (alt_inr : Assertion (Σ ▻ xr∷τ))
+  | match_list
       {σ : Ty} (s : Term Σ (ty.list σ)) (alt_nil : Assertion Σ) (xh xt : LVar)
       (alt_cons : Assertion (Σ ▻ xh∷σ ▻ xt∷ty.list σ))
-  | asn_match_prod
+  | match_prod
       {σ1 σ2 : Ty} (s : Term Σ (ty.prod σ1 σ2))
       (xl xr : LVar) (rhs : Assertion (Σ ▻ xl∷σ1 ▻ xr∷σ2))
-  | asn_match_tuple
+  | match_tuple
       {σs : Ctx Ty} {Δ : LCtx} (s : Term Σ (ty.tuple σs))
       (p : TuplePat σs Δ) (rhs : Assertion (Σ ▻▻ Δ))
-  | asn_match_record
+  | match_record
       {R : recordi} {Δ : LCtx} (s : Term Σ (ty.record R))
       (p : RecordPat (recordf_ty R) Δ) (rhs : Assertion (Σ ▻▻ Δ))
-  | asn_match_union
+  | match_union
       {U : unioni} (s : Term Σ (ty.union U))
       (alt__ctx : forall (K : unionk U), LCtx)
       (alt__pat : forall (K : unionk U), Pattern (alt__ctx K) (unionk_ty U K))
       (alt__rhs : forall (K : unionk U), Assertion (Σ ▻▻ alt__ctx K))
-  | asn_sep  (a1 a2 : Assertion Σ)
-  | asn_or   (a1 a2 : Assertion Σ)
-  | asn_exist (ς : LVar) (τ : Ty) (a : Assertion (Σ ▻ ς∷τ))
-  | asn_debug.
-  Bind Scope asn_scope with Assertion.
+  | sep  (A1 A2 : Assertion Σ)
+  | or   (A1 A2 : Assertion Σ)
+  | exist (ς : LVar) (τ : Ty) (a : Assertion (Σ ▻ ς∷τ))
+  | debug.
 
-  Arguments asn_match_enum [_] E _ _.
-  Arguments asn_match_sum [_] σ τ _ _ _.
-  Arguments asn_match_list [_] {σ} s alt_nil xh xt alt_cons.
-  Arguments asn_match_prod [_] {σ1 σ2} s xl xr rhs.
-  Arguments asn_match_tuple [_] {σs Δ} s p rhs.
-  Arguments asn_match_record [_] R {Δ} s p rhs.
-  Arguments asn_match_union [_] U s alt__ctx alt__pat alt__rhs.
-  Arguments asn_exist [_] _ _ _.
-  Arguments asn_debug {_}.
+  #[global] Arguments match_enum [_] E _ _.
+  #[global] Arguments match_sum [_] σ τ _ _ _.
+  #[global] Arguments match_list [_] {σ} s alt_nil xh xt alt_cons.
+  #[global] Arguments match_prod [_] {σ1 σ2} s xl xr rhs.
+  #[global] Arguments match_tuple [_] {σs Δ} s p rhs.
+  #[global] Arguments match_record [_] R {Δ} s p rhs.
+  #[global] Arguments match_union [_] U s alt__ctx alt__pat alt__rhs.
+  #[global] Arguments exist [_] _ _ _.
+  #[global] Arguments debug {_}.
 
-  Notation asn_bool b := (asn_formula (formula_bool b)).
-  Notation asn_prop Σ P := (asn_formula (@formula_prop Σ Σ (sub_id Σ) P)).
-  Notation asn_eq t1 t2 := (asn_formula (formula_eq t1 t2)).
-  Notation asn_true := (asn_bool (term_val ty.bool true)).
-  Notation asn_false := (asn_bool (term_val ty.bool false)).
+  Fixpoint exs {Σ} Δ : Assertion (Σ ▻▻ Δ) -> Assertion Σ :=
+    match Δ return Assertion (Σ ▻▻ Δ) -> Assertion Σ with
+    | ctx.nil => fun A => A
+    | ctx.snoc Γ (x :: τ) =>
+      fun A =>
+        @exs Σ Γ (exist x τ A)
+    end.
 
   #[export] Instance sub_assertion : Subst Assertion :=
-    fix sub_assertion {Σ1} (a : Assertion Σ1) {Σ2} (ζ : Sub Σ1 Σ2) {struct a} : Assertion Σ2 :=
-      match a with
-      | asn_formula fml => asn_formula (subst fml ζ)
-      | asn_chunk c => asn_chunk (subst c ζ)
-      | asn_chunk_angelic c => asn_chunk_angelic (subst c ζ)
-      | asn_if b a1 a2 => asn_if (subst b ζ) (sub_assertion a1 ζ) (sub_assertion a2 ζ)
-      | asn_match_enum E k alts =>
-        asn_match_enum E (subst k ζ) (fun z => sub_assertion (alts z) ζ)
-      | asn_match_sum σ τ t xl al xr ar =>
-        asn_match_sum σ τ (subst t ζ) xl (sub_assertion al (sub_up1 ζ)) xr (sub_assertion ar (sub_up1 ζ))
-      | asn_match_list s anil xh xt acons =>
-        asn_match_list (subst s ζ) (sub_assertion anil ζ) xh xt (sub_assertion acons (sub_up1 (sub_up1 ζ)))
-      | asn_match_prod s xl xr asn =>
-        asn_match_prod (subst s ζ) xl xr (sub_assertion asn (sub_up1 (sub_up1 ζ)))
-      | asn_match_tuple s p rhs =>
-        asn_match_tuple (subst s ζ) p (sub_assertion rhs (sub_up ζ _))
-      | asn_match_record R s p rhs =>
-        asn_match_record R (subst s ζ) p (sub_assertion rhs (sub_up ζ _))
-      | asn_match_union U s ctx pat rhs =>
-        asn_match_union U (subst s ζ) ctx pat (fun K => sub_assertion (rhs K) (sub_up ζ _))
-      | asn_sep a1 a2 => asn_sep (sub_assertion a1 ζ) (sub_assertion a2 ζ)
-      | asn_or a1 a2  => asn_sep (sub_assertion a1 ζ) (sub_assertion a2 ζ)
-      | asn_exist ς τ a => asn_exist ς τ (sub_assertion a (sub_up1 ζ))
-      | asn_debug => asn_debug
+    fix sub_assertion {Σ1} (A : Assertion Σ1) {Σ2} (ζ : Sub Σ1 Σ2) {struct A} : Assertion Σ2 :=
+      match A with
+      | formula fml => formula (subst fml ζ)
+      | chunk c => chunk (subst c ζ)
+      | chunk_angelic c => chunk_angelic (subst c ζ)
+      | match_bool b A1 A2 => match_bool (subst b ζ) (sub_assertion A1 ζ) (sub_assertion A2 ζ)
+      | match_enum E k alts =>
+        match_enum E (subst k ζ) (fun z => sub_assertion (alts z) ζ)
+      | match_sum σ τ t xl al xr ar =>
+        match_sum σ τ (subst t ζ) xl (sub_assertion al (sub_up1 ζ)) xr (sub_assertion ar (sub_up1 ζ))
+      | match_list s anil xh xt acons =>
+        match_list (subst s ζ) (sub_assertion anil ζ) xh xt (sub_assertion acons (sub_up1 (sub_up1 ζ)))
+      | match_prod s xl xr A =>
+        match_prod (subst s ζ) xl xr (sub_assertion A (sub_up1 (sub_up1 ζ)))
+      | match_tuple s p A =>
+        match_tuple (subst s ζ) p (sub_assertion A (sub_up ζ _))
+      | match_record R s p A =>
+        match_record R (subst s ζ) p (sub_assertion A (sub_up ζ _))
+      | match_union U s ctx pat rhs =>
+        match_union U (subst s ζ) ctx pat (fun K => sub_assertion (rhs K) (sub_up ζ _))
+      | sep A1 A2 => sep (sub_assertion A1 ζ) (sub_assertion A2 ζ)
+      | or A1 A2  => sep (sub_assertion A1 ζ) (sub_assertion A2 ζ)
+      | exist ς τ A => exist ς τ (sub_assertion A (sub_up1 ζ))
+      | debug => debug
       end.
 
-  (* This instance is only used for linting contracts. *)
+  (* This instance is only used for linting contracts, so we only used it as an
+     instance locally. *)
   Import option.notations.
-  #[export] Instance OccursCheckAssertion :
+  #[local] Instance OccursCheckAssertion :
     OccursCheck Assertion :=
     fix occurs Σ b (bIn : b ∈ Σ) (asn : Assertion Σ) : option (Assertion (Σ - b)) :=
       match asn with
-      | asn_formula fml => option.map (@asn_formula _) (occurs_check bIn fml)
-      | asn_chunk c     => option.map (@asn_chunk _) (occurs_check bIn c)
-      | asn_chunk_angelic c => option.map (@asn_chunk_angelic _) (occurs_check bIn c)
-      | asn_if b a1 a2  =>
+      | formula fml => option.map (@formula _) (occurs_check bIn fml)
+      | chunk c     => option.map (@chunk _) (occurs_check bIn c)
+      | chunk_angelic c => option.map (@chunk_angelic _) (occurs_check bIn c)
+      | match_bool b a1 a2  =>
           b'  <- occurs_check bIn b;;
           a1' <- occurs _ _ bIn a1 ;;
           a2' <- occurs _ _ bIn a2 ;;
-          Some (asn_if b' a1' a2')
-      | asn_match_enum E k alts => None (* TODO *)
-      | asn_match_sum σ τ s xl alt_inl xr alt_inr =>
+          Some (match_bool b' a1' a2')
+      | match_enum E k alts => None (* TODO *)
+      | match_sum σ τ s xl alt_inl xr alt_inr =>
           s'   <- occurs_check bIn s ;;
           inl' <- occurs (Σ ▻ xl∷σ) b (ctx.in_succ bIn) alt_inl ;;
           inr' <- occurs (Σ ▻ xr∷τ) b (ctx.in_succ bIn) alt_inr ;;
-          Some (asn_match_sum σ τ s' xl inl' xr inr')
-      | @asn_match_list _ σ s alt_nil xh xt alt_cons => None (* TODO *)
-      | @asn_match_prod _ σ1 σ2 s xl xr rhs => None (* TODO *)
-      | @asn_match_tuple _ σs Δ s p rhs => None (* TODO *)
-      | @asn_match_record _ R4 Δ s p rhs => None (* TODO *)
-      | asn_match_union U s alt__ctx alt__pat alt__rhs => None (* TODO *)
-      | asn_sep a1 a2 =>
-          a1' <- occurs _ _ bIn a1 ;;
-          a2' <- occurs _ _ bIn a2 ;;
-          Some (asn_sep a1' a2')
-      | asn_or a1 a2  =>
-          a1' <- occurs _ _ bIn a1 ;;
-          a2' <- occurs _ _ bIn a2 ;;
-          Some (asn_or a1' a2')
-      | asn_exist ς τ a => option_map (@asn_exist _ ς τ) (occurs _ _ (ctx.in_succ bIn) a)
-      | asn_debug => Some asn_debug
+          Some (match_sum σ τ s' xl inl' xr inr')
+      | @match_list _ σ s alt_nil xh xt alt_cons => None (* TODO *)
+      | @match_prod _ σ1 σ2 s xl xr rhs => None (* TODO *)
+      | @match_tuple _ σs Δ s p rhs => None (* TODO *)
+      | @match_record _ R4 Δ s p rhs => None (* TODO *)
+      | match_union U s alt__ctx alt__pat alt__rhs => None (* TODO *)
+      | sep A1 A2 =>
+          A1' <- occurs _ _ bIn A1 ;;
+          A2' <- occurs _ _ bIn A2 ;;
+          Some (sep A1' A2')
+      | or A1 A2  =>
+          A1' <- occurs _ _ bIn A1 ;;
+          A2' <- occurs _ _ bIn A2 ;;
+          Some (or A1' A2')
+      | exist ς τ A => option_map (@exist _ ς τ) (occurs _ _ (ctx.in_succ bIn) A)
+      | debug => Some debug
       end.
+
+  Fixpoint is_pure {Σ} (a : Assertion Σ) : bool :=
+    match a with
+    | formula fml => true
+    | chunk c => false
+    | chunk_angelic c => false
+    | match_bool b A1 A2 => is_pure A1 && is_pure A2
+    | match_enum E k alts => List.forallb (fun K => is_pure (alts K)) (finite.enum _)
+    | match_sum σ τ s xl alt_inl xr alt_inr => is_pure alt_inl && is_pure alt_inr
+    | match_list s alt_nil xh xt alt_cons => is_pure alt_nil && is_pure alt_cons
+    | match_prod s xl xr rhs => is_pure rhs
+    | match_tuple s p rhs => is_pure rhs
+    | match_record R s p rhs => is_pure rhs
+    | match_union U s alt__ctx alt__pat alt__rhs => List.forallb (fun K => is_pure (alt__rhs K)) (finite.enum _)
+    | sep A1 A2 => is_pure A1 && is_pure A2
+    | or A1 A2  => is_pure A1 && is_pure A2
+    | exist ς τ A => is_pure A
+    | debug => true
+  end.
+
+  Section Interpretation.
+    Import sep.notations.
+
+    Fixpoint interpret_pure {Σ} (a : Assertion Σ) (ι : Valuation Σ) : Prop :=
+      match a with
+      | formula F => inst F ι
+      | chunk c => False
+      | chunk_angelic c => False
+      | match_bool b A1 A2 =>
+        if inst (A := Val ty.bool) b ι
+        then interpret_pure A1 ι
+        else interpret_pure A2 ι
+      | match_enum E k alts => interpret_pure (alts (inst (T := fun Σ => Term Σ _) k ι)) ι
+      | match_sum σ τ s xl alt_inl xr alt_inr =>
+        match inst (T := fun Σ => Term Σ _) s ι with
+        | inl v => interpret_pure alt_inl (ι ► (xl∷σ ↦ v))
+        | inr v => interpret_pure alt_inr (ι ► (xr∷τ ↦ v))
+        end
+      | match_list s alt_nil xh xt alt_cons =>
+        match inst (T := fun Σ => Term Σ _) s ι with
+        | nil        => interpret_pure alt_nil ι
+        | cons vh vt => interpret_pure alt_cons (ι ► (xh∷_ ↦ vh) ► (xt∷ty.list _ ↦ vt))
+        end
+      | match_prod s xl xr rhs =>
+        match inst (T := fun Σ => Term Σ _) s ι with
+        | (vl,vr)    => interpret_pure rhs (ι ► (xl∷_ ↦ vl) ► (xr∷_ ↦ vr))
+        end
+      | match_tuple s p rhs =>
+        let t := inst (T := fun Σ => Term Σ _) s ι in
+        let ι' := tuple_pattern_match_val p t in
+        interpret_pure rhs (ι ►► ι')
+      | match_record R s p rhs =>
+        let t := inst (T := fun Σ => Term Σ _) s ι in
+        let ι' := record_pattern_match_val p t in
+        interpret_pure rhs (ι ►► ι')
+      | match_union U s alt__ctx alt__pat alt__rhs =>
+        let t := inst (T := fun Σ => Term Σ _) s ι in
+        let (K , v) := unionv_unfold U t in
+        let ι' := pattern_match_val (alt__pat K) v in
+        interpret_pure (alt__rhs K) (ι ►► ι')
+      | sep A1 A2 => interpret_pure A1 ι /\ interpret_pure A2 ι
+      | or A1 A2  => interpret_pure A1 ι \/ interpret_pure A2 ι
+      | exist ς τ A => exists (v : Val τ), interpret_pure A (ι ► (ς∷τ ↦ v))
+      | debug => True
+    end.
+
+    Context {HProp} `{PI : PredicateDef HProp}.
+
+    Fixpoint interpret {Σ} (A : Assertion Σ) (ι : Valuation Σ) : HProp :=
+      match A with
+      | formula F => !!(inst F ι) ∧ lemp
+      | chunk c => interpret_chunk c ι
+      | chunk_angelic c => interpret_chunk c ι
+      | match_bool b a1 a2 =>
+        if inst (A := Val ty.bool) b ι
+        then interpret a1 ι
+        else interpret a2 ι
+      | match_enum E k alts => interpret (alts (inst (T := fun Σ => Term Σ _) k ι)) ι
+      | match_sum σ τ s xl alt_inl xr alt_inr =>
+        match inst (T := fun Σ => Term Σ _) s ι with
+        | inl v => interpret alt_inl (ι ► (xl∷σ ↦ v))
+        | inr v => interpret alt_inr (ι ► (xr∷τ ↦ v))
+        end
+      | match_list s alt_nil xh xt alt_cons =>
+        match inst (T := fun Σ => Term Σ _) s ι with
+        | nil        => interpret alt_nil ι
+        | cons vh vt => interpret alt_cons (ι ► (xh∷_ ↦ vh) ► (xt∷ty.list _ ↦ vt))
+        end
+      | match_prod s xl xr rhs =>
+        match inst (T := fun Σ => Term Σ _) s ι with
+        | (vl,vr)    => interpret rhs (ι ► (xl∷_ ↦ vl) ► (xr∷_ ↦ vr))
+        end
+      | match_tuple s p rhs =>
+        let t := inst (T := fun Σ => Term Σ _) s ι in
+        let ι' := tuple_pattern_match_val p t in
+        interpret rhs (ι ►► ι')
+      | match_record R s p rhs =>
+        let t := inst (T := fun Σ => Term Σ _) s ι in
+        let ι' := record_pattern_match_val p t in
+        interpret rhs (ι ►► ι')
+      | match_union U s alt__ctx alt__pat alt__rhs =>
+        let t := inst (T := fun Σ => Term Σ _) s ι in
+        let (K , v) := unionv_unfold U t in
+        let ι' := pattern_match_val (alt__pat K) v in
+        interpret (alt__rhs K) (ι ►► ι')
+      | sep A1 A2 => interpret A1 ι ∗ interpret A2 ι
+      | or A1 A2  => interpret A1 ι ∨ interpret A2 ι
+      | exist ς τ A => ∃ (v : Val τ), interpret A (ι ► (ς∷τ ↦ v))
+      | debug => lemp
+    end.
+
+    Import sep.instances.
+
+    Lemma interpret_pure_equiv {Σ} (a : Assertion Σ) (a_pure : is_pure a = true) :
+      forall (ι : Valuation Σ),
+        interpret a ι ⊣⊢ !!(interpret_pure a ι).
+    Proof.
+      induction a; cbn in *; intros ι; try discriminate a_pure.
+      - now rewrite lemp_true, land_true.
+      - apply andb_true_iff in a_pure. destruct a_pure.
+        destruct (inst b ι); auto.
+      - apply H. rewrite List.forallb_forall in a_pure. apply a_pure.
+        apply base.elem_of_list_In. apply finite.elem_of_enum.
+      - apply andb_true_iff in a_pure. destruct a_pure.
+        destruct (inst s ι); auto.
+      - apply andb_true_iff in a_pure. destruct a_pure.
+        destruct (inst s ι); auto.
+      - destruct (inst s ι); auto.
+      - apply IHa; auto.
+      - apply IHa; auto.
+      - destruct (unionv_unfold U (inst s ι)).
+        apply H. rewrite List.forallb_forall in a_pure. apply a_pure.
+        apply base.elem_of_list_In. apply finite.elem_of_enum.
+      - apply andb_true_iff in a_pure. destruct a_pure.
+        rewrite IHa1, IHa2; auto. now rewrite lprop_sep_distr.
+      - apply andb_true_iff in a_pure. destruct a_pure.
+        rewrite IHa1, IHa2; auto. now rewrite lprop_or_distr.
+      - setoid_rewrite IHa; auto.
+        now rewrite lprop_exists_comm.
+      - apply lemp_true.
+    Qed.
+
+  End Interpretation.
+
+  Module notations.
+    Open Scope asn_scope.
+
+    Notation "r ↦ val" := (chunk (chunk_ptsreg r val)) (at level 70) : asn_scope.
+    Notation "P ∗ Q" := (sep P Q) : asn_scope.
+    Notation "∃ w , A" := (exist w _ A) (at level 79, right associativity) : asn_scope.
+    Notation "P ∨ Q" := (or P Q) : asn_scope.
+    Notation "⊤" := (formula (formula_bool (term_val ty.bool true))) : asn_scope.
+    Notation "⊥" := (formula (formula_bool (term_val ty.bool false))) : asn_scope.
+    Notation "'if:' c 'then' A1 'else' A2" := (match_bool c A1 A2)
+      (at level 200, format
+       "'[hv' 'if:'  c  '/' '[' 'then'  A1  ']' '/' '[' 'else'  A2 ']' ']'"
+      ) : asn_scope.
+    Notation "x = y" := (formula (formula_eq x y)) : asn_scope.
+    Notation "x < y" := (formula (formula_lt x y)) : asn_scope.
+    Notation "x <= y" := (formula (formula_le x y)) : asn_scope.
+    Notation "x > y" := (formula (formula_gt x y)) : asn_scope.
+    Notation "x >= y" := (formula (formula_ge x y)) : asn_scope.
+
+  End notations.
+
+End asn.
+Export asn ( Assertion ).
+Bind Scope asn_scope with Assertion.
+
+Section Contracts.
+  #[local] Existing Instance OccursCheckAssertion.
 
   Record SepContract (Δ : PCtx) (τ : Ty) : Type :=
     MkSepContract
@@ -169,7 +344,7 @@ Module Type AssertionsOn
         sep_contract_postcondition    : Assertion (sep_contract_logic_variables ▻ sep_contract_result∷τ);
       }.
 
-  Arguments MkSepContract : clear implicits.
+  #[global] Arguments MkSepContract : clear implicits.
 
   Record Lemma (Δ : PCtx) : Type :=
     MkLemma
@@ -179,7 +354,7 @@ Module Type AssertionsOn
         lemma_postcondition    : Assertion lemma_logic_variables;
       }.
 
-  Arguments MkLemma : clear implicits.
+  #[global] Arguments MkLemma : clear implicits.
 
   Definition lint_contract {Δ σ} (c : SepContract Δ σ) : bool :=
     match c with
@@ -261,80 +436,9 @@ Module Type AssertionsOn
 
   End Experimental.
 
-  Import sep.notations.
-
-  Class PredicateDef (HProp : SepLogic) : Type :=
-    { lptsreg    : forall {σ : Ty}, 𝑹𝑬𝑮 σ -> Val σ -> HProp;
-      luser      : forall (p : 𝑯), Env Val (𝑯_Ty p) -> HProp;
-      lduplicate : forall (p : 𝑯) (ts : Env Val (𝑯_Ty p)),
-        is_duplicable p = true ->
-        @luser p ts ⊢ @luser p ts ∗ @luser p ts;
-    }.
-  Arguments luser {_ _} p _.
-
   Section ContractInt.
 
     Context {HProp} `{PI : PredicateDef HProp}.
-
-    Fixpoint interpret_chunk {Σ} (c : Chunk Σ) (ι : Valuation Σ) {struct c} : HProp :=
-      match c with
-      | chunk_user p ts => luser p (inst ts ι)
-      | chunk_ptsreg r t => lptsreg r (inst t ι)
-      | chunk_conj c1 c2 => interpret_chunk c1 ι ∗ interpret_chunk c2 ι
-      | chunk_wand c1 c2 => interpret_chunk c1 ι -∗ interpret_chunk c2 ι
-      end.
-
-    Fixpoint interpret_scchunk (c : SCChunk) : HProp :=
-      match c with
-      | scchunk_user p vs => luser p vs
-      | scchunk_ptsreg r v => lptsreg r v
-      | scchunk_conj c1 c2 => interpret_scchunk c1 ∗ interpret_scchunk c2
-      | scchunk_wand c1 c2 => interpret_scchunk c1 -∗ interpret_scchunk c2
-      end.
-
-    Definition interpret_scheap : SCHeap -> HProp :=
-      List.fold_right (fun c h => interpret_scchunk c ∗ h) lemp.
-    Arguments interpret_scheap !h.
-
-    Fixpoint interpret_assertion {Σ} (a : Assertion Σ) (ι : Valuation Σ) : HProp :=
-      match a with
-      | asn_formula fml => !!(inst fml ι) ∧ lemp
-      | asn_chunk c => interpret_chunk c ι
-      | asn_chunk_angelic c => interpret_chunk c ι
-      | asn_if b a1 a2 => if inst (A := Val ty.bool) b ι then interpret_assertion a1 ι else interpret_assertion a2 ι
-      | asn_match_enum E k alts => interpret_assertion (alts (inst (T := fun Σ => Term Σ _) k ι)) ι
-      | asn_match_sum σ τ s xl alt_inl xr alt_inr =>
-        match inst (T := fun Σ => Term Σ _) s ι with
-        | inl v => interpret_assertion alt_inl (ι ► (xl∷σ ↦ v))
-        | inr v => interpret_assertion alt_inr (ι ► (xr∷τ ↦ v))
-        end
-      | asn_match_list s alt_nil xh xt alt_cons =>
-        match inst (T := fun Σ => Term Σ _) s ι with
-        | nil        => interpret_assertion alt_nil ι
-        | cons vh vt => interpret_assertion alt_cons (ι ► (xh∷_ ↦ vh) ► (xt∷ty.list _ ↦ vt))
-        end
-      | asn_match_prod s xl xr rhs =>
-        match inst (T := fun Σ => Term Σ _) s ι with
-        | (vl,vr)    => interpret_assertion rhs (ι ► (xl∷_ ↦ vl) ► (xr∷_ ↦ vr))
-        end
-      | asn_match_tuple s p rhs =>
-        let t := inst (T := fun Σ => Term Σ _) s ι in
-        let ι' := tuple_pattern_match_val p t in
-        interpret_assertion rhs (ι ►► ι')
-      | asn_match_record R s p rhs =>
-        let t := inst (T := fun Σ => Term Σ _) s ι in
-        let ι' := record_pattern_match_val p t in
-        interpret_assertion rhs (ι ►► ι')
-      | asn_match_union U s alt__ctx alt__pat alt__rhs =>
-        let t := inst (T := fun Σ => Term Σ _) s ι in
-        let (K , v) := unionv_unfold U t in
-        let ι' := pattern_match_val (alt__pat K) v in
-        interpret_assertion (alt__rhs K) (ι ►► ι')
-      | asn_sep a1 a2 => interpret_assertion a1 ι ∗ interpret_assertion a2 ι
-      | asn_or a1 a2  => interpret_assertion a1 ι ∨ interpret_assertion a2 ι
-      | asn_exist ς τ a => ∃ (v : Val τ), interpret_assertion a (ι ► (ς∷τ ↦ v))
-      | asn_debug => lemp
-    end.
 
     Definition inst_contract_localstore {Δ τ} (c : SepContract Δ τ)
       (ι : Valuation (sep_contract_logic_variables c)) : CStore Δ :=
@@ -342,102 +446,13 @@ Module Type AssertionsOn
 
     Definition interpret_contract_precondition {Δ τ} (c : SepContract Δ τ)
       (ι : Valuation (sep_contract_logic_variables c)) : HProp :=
-      interpret_assertion (sep_contract_precondition c) ι.
+      interpret (sep_contract_precondition c) ι.
 
     Definition interpret_contract_postcondition {Δ τ} (c : SepContract Δ τ)
       (ι : Valuation (sep_contract_logic_variables c)) (result : Val τ) : HProp :=
-        interpret_assertion (sep_contract_postcondition c) (env.snoc ι (sep_contract_result c ∷ τ) result).
-
-    Fixpoint is_pure {Σ} (a : Assertion Σ) : bool :=
-      match a with
-      | asn_formula fml => true
-      | asn_chunk c => false
-      | asn_chunk_angelic c => false
-      | asn_if b a1 a2 => is_pure a1 && is_pure a2
-      | asn_match_enum E k alts => List.forallb (fun K => is_pure (alts K)) (finite.enum _)
-      | asn_match_sum σ τ s xl alt_inl xr alt_inr => is_pure alt_inl && is_pure alt_inr
-      | asn_match_list s alt_nil xh xt alt_cons => is_pure alt_nil && is_pure alt_cons
-      | asn_match_prod s xl xr rhs => is_pure rhs
-      | asn_match_tuple s p rhs => is_pure rhs
-      | asn_match_record R s p rhs => is_pure rhs
-      | asn_match_union U s alt__ctx alt__pat alt__rhs => List.forallb (fun K => is_pure (alt__rhs K)) (finite.enum _)
-      | asn_sep a1 a2 => is_pure a1 && is_pure a2
-      | asn_or a1 a2  => is_pure a1 && is_pure a2
-      | asn_exist ς τ a => is_pure a
-      | asn_debug => true
-    end.
-
-    Fixpoint interpret_assertion_pure {Σ} (a : Assertion Σ) (ι : Valuation Σ) : Prop :=
-      match a with
-      | asn_formula fml => inst fml ι
-      | asn_chunk c => False
-      | asn_chunk_angelic c => False
-      | asn_if b a1 a2 => if inst (A := Val ty.bool) b ι then interpret_assertion_pure a1 ι else interpret_assertion_pure a2 ι
-      | asn_match_enum E k alts => interpret_assertion_pure (alts (inst (T := fun Σ => Term Σ _) k ι)) ι
-      | asn_match_sum σ τ s xl alt_inl xr alt_inr =>
-        match inst (T := fun Σ => Term Σ _) s ι with
-        | inl v => interpret_assertion_pure alt_inl (ι ► (xl∷σ ↦ v))
-        | inr v => interpret_assertion_pure alt_inr (ι ► (xr∷τ ↦ v))
-        end
-      | asn_match_list s alt_nil xh xt alt_cons =>
-        match inst (T := fun Σ => Term Σ _) s ι with
-        | nil        => interpret_assertion_pure alt_nil ι
-        | cons vh vt => interpret_assertion_pure alt_cons (ι ► (xh∷_ ↦ vh) ► (xt∷ty.list _ ↦ vt))
-        end
-      | asn_match_prod s xl xr rhs =>
-        match inst (T := fun Σ => Term Σ _) s ι with
-        | (vl,vr)    => interpret_assertion_pure rhs (ι ► (xl∷_ ↦ vl) ► (xr∷_ ↦ vr))
-        end
-      | asn_match_tuple s p rhs =>
-        let t := inst (T := fun Σ => Term Σ _) s ι in
-        let ι' := tuple_pattern_match_val p t in
-        interpret_assertion_pure rhs (ι ►► ι')
-      | asn_match_record R s p rhs =>
-        let t := inst (T := fun Σ => Term Σ _) s ι in
-        let ι' := record_pattern_match_val p t in
-        interpret_assertion_pure rhs (ι ►► ι')
-      | asn_match_union U s alt__ctx alt__pat alt__rhs =>
-        let t := inst (T := fun Σ => Term Σ _) s ι in
-        let (K , v) := unionv_unfold U t in
-        let ι' := pattern_match_val (alt__pat K) v in
-        interpret_assertion_pure (alt__rhs K) (ι ►► ι')
-      | asn_sep a1 a2 => interpret_assertion_pure a1 ι /\ interpret_assertion_pure a2 ι
-      | asn_or a1 a2  => interpret_assertion_pure a1 ι \/ interpret_assertion_pure a2 ι
-      | asn_exist ς τ a => exists (v : Val τ), interpret_assertion_pure a (ι ► (ς∷τ ↦ v))
-      | asn_debug => True
-    end.
-
-    Import sep.instances.
-
-    Lemma interpret_assertion_pure_equiv {Σ} (a : Assertion Σ) (a_pure : is_pure a = true) :
-      forall (ι : Valuation Σ),
-        interpret_assertion a ι ⊣⊢ !!(interpret_assertion_pure a ι).
-    Proof.
-      induction a; cbn in *; intros ι; try discriminate a_pure.
-      - now rewrite lemp_true, land_true.
-      - apply andb_true_iff in a_pure. destruct a_pure.
-        destruct (inst b ι); auto.
-      - apply H. rewrite List.forallb_forall in a_pure. apply a_pure.
-        apply base.elem_of_list_In. apply finite.elem_of_enum.
-      - apply andb_true_iff in a_pure. destruct a_pure.
-        destruct (inst s ι); auto.
-      - apply andb_true_iff in a_pure. destruct a_pure.
-        destruct (inst s ι); auto.
-      - destruct (inst s ι); auto.
-      - apply IHa; auto.
-      - apply IHa; auto.
-      - destruct (unionv_unfold U (inst s ι)).
-        apply H. rewrite List.forallb_forall in a_pure. apply a_pure.
-        apply base.elem_of_list_In. apply finite.elem_of_enum.
-      - apply andb_true_iff in a_pure. destruct a_pure.
-        rewrite IHa1, IHa2; auto. now rewrite lprop_sep_distr.
-      - apply andb_true_iff in a_pure. destruct a_pure.
-        rewrite IHa1, IHa2; auto. now rewrite lprop_or_distr.
-      - setoid_rewrite IHa; auto.
-        now rewrite lprop_exists_comm.
-      - apply lemp_true.
-    Qed.
+        interpret (sep_contract_postcondition c) (env.snoc ι (sep_contract_result c ∷ τ) result).
 
   End ContractInt.
 
+End Contracts.
 End AssertionsOn.
