theories/Syntax/Predicates.v
@@ -31,6 +31,7 @@ From Katamaran Require Import
      Context
      Environment
      Prelude
+     Sep.Logic
      Base.
 
 From Equations Require Import
@@ -67,8 +68,20 @@ Module Type HeapPredicateKit (Import B : Base).
 
 End HeapPredicateKit.
 
+Module Type PredicateMixin (Import B : Base) (Import PP : PurePredicateKit B) (Import HP : HeapPredicateKit B).
+  Import sep.notations.
+  Class PredicateDef (HProp : SepLogic) : Type :=
+  { lptsreg    : forall {σ : Ty}, 𝑹𝑬𝑮 σ -> Val σ -> HProp;
+    luser      : forall (p : 𝑯), Env Val (𝑯_Ty p) -> HProp;
+    lduplicate : forall (p : 𝑯) (ts : Env Val (𝑯_Ty p)),
+      is_duplicable p = true ->
+      @luser p ts ⊢ @luser p ts ∗ @luser p ts;
+  }.
+  Arguments luser {_ _} p _.
+End PredicateMixin.
+
 Module Type PredicateKit (B : Base) :=
-  PurePredicateKit B <+ HeapPredicateKit B.
+  PurePredicateKit B <+ HeapPredicateKit B <+ PredicateMixin B.
 
 Module DefaultPurePredicateKit (Import B : Base) <: PurePredicateKit B.
 
